

对数运算测试题

1. $\frac{\log_3 \left(\frac{27}{\log_3 8} \right)}{\log_3 3} + \log_3 \left(\frac{\log_3 8}{4} \right) + \log_3 4 = \underline{\hspace{2cm}}$
2. $\log_{(7+3)} (100(7+3)^2) - \log_{(7+3)} (7+3)^2 = \underline{\hspace{2cm}}$
3. $\frac{\log (2^{\log_2 10})^{125}}{\frac{\log_2 e^{\ln 5}}{\log_2 (2 \times 5)}} = \underline{\hspace{2cm}}$
4. $\log_{(2^{\log_2 (4(2+3)) - \log_2 (2+3)})} (2 \times 2) = \underline{\hspace{2cm}}$
5. $\frac{\log_{((1+2)^2)} 10}{\log_{((1+2)^2)} \log_5 5^{10}} = \underline{\hspace{2cm}}$
6. $\frac{1}{\log_{\left(\frac{e^4}{3 \times 3}\right)} e} + \frac{1}{\log_{(3 \times 3)} e} = \underline{\hspace{2cm}}$
7. $\frac{\frac{\lg 1000}{\lg \left(\frac{6}{3} \times 2\right)}}{\log_{\left(\frac{6}{3} \times 2\right)} e^{\ln 10}} = \underline{\hspace{2cm}}$
8. $\log \left(\frac{\log_{(1+1)} 5}{e^{\frac{\log_{(1+1)} e}{e}}} \right) (14 + 11) = \underline{\hspace{2cm}}$
9. $\log_{(2^{\log_2 4} + 1)} (5 \log_2 9) - \log_{(2^{\log_2 4} + 1)} \log_2 9 = \underline{\hspace{2cm}}$
10. $\log_3 ((5+4)(3+2+3-3)) - \log_{(3^{\log_3 3})} (3+2) = \underline{\hspace{2cm}}$
11. $\frac{\frac{1}{2} \frac{\lg 5^2}{\log_{(2 \times 2)} e^{\ln 5}}}{\frac{\log_{(2 \times 2)} 10}{\log_{(2 \times 2)} 10}} = \underline{\hspace{2cm}}$
12. $\frac{\log_{(2^3)} 2}{\log_{(2^3)} \left(\frac{2}{5} \right) + \log_{(2^3)} 5} = \underline{\hspace{2cm}}$
13. $\frac{\frac{\log_3 10}{\log_3 \left(\frac{1 \times 5 + 1 \times 5}{5} \right)}}{\log_{(1+1)} (8+2)} = \underline{\hspace{2cm}}$
14. $\frac{\frac{\log_2 2}{1}}{\log_{(1+4)} \left(\frac{7^5}{4} (\lg 2 \lg 5 + \lg^2 2 + \lg 5) \right)} = \underline{\hspace{2cm}}$
15. $\lg \left(\frac{236+764}{10^3} \right) + \frac{\log_{(3^2)} 10^3}{\log_{(3^2)} 10} = \underline{\hspace{2cm}}$
16. $\frac{1}{\log_{(3 \times 9)} \left(\frac{3}{3 \times 3} \right) + \log_{(3 \times 9)} (3 \times 3)} = \underline{\hspace{2cm}}$

17. $\frac{\log_3 (64\frac{1}{4})}{\log_3 4} - \log_4 (\frac{1}{4} \times 4^3) - \log_4 4^3 = \underline{\hspace{2cm}}$
18. $\log_{(2+3)} \left(\frac{25}{(2+3)^I} \right) + \log_{(2+3)} (2+3)^1 = \underline{\hspace{2cm}}$
19. $\frac{\log_2 (3 \times 3)}{\log (2(\lg 2 \lg 5 + \lg^2 2 + \lg 5))} 3^{\log_3 3} = \underline{\hspace{2cm}}$
20. $\log_5 (5 (\lg 2 \lg 2 + \lg 5 \lg 5 + 2 \lg 5 \lg 2) \frac{1}{4}) - \log_5 (\frac{1}{4}) = \underline{\hspace{2cm}}$
21. $\frac{\frac{\log_3 e^{\ln 16}}{\log_3 3}}{\frac{\log (2^2)^2}{\log (2^2)^3}} = \underline{\hspace{2cm}}$
22. $\frac{\log_5 (9 \times 4)}{\log_5 3} - \log_3 (\frac{4}{3 \times 3}) + \log_3 (3 \times 3) = \underline{\hspace{2cm}}$
23. $\frac{\log_5 (5^{\log_5 4 \times 5^3}) - \log (\frac{15}{2}) 5^3}{\frac{\ln 2}{\ln 5}} = \underline{\hspace{2cm}}$
24. $\frac{\frac{\lg 10 \lg 10}{\lg (2^2(3+2)) - \lg (3+2)}}{\frac{1}{\lg 2^2}} = \underline{\hspace{2cm}}$
25. $\log_2 \left(\frac{2^{\frac{\log_2 5^{\log_5 2}}{\log_2 2}}}{3 \times 2} \right) + \log_2 (3 \times 2) = \underline{\hspace{2cm}}$
26. $\frac{1}{\log (\frac{3000 \times 1}{4 \times 1} \times 2) (\frac{40}{3})} - \log (\frac{40}{3})^2 = \underline{\hspace{2cm}}$
27. $\log_{(2^{\log_2 2})} (4 (1+1)) - \log_{(2^{\log_2 2})} (1+1) = \underline{\hspace{2cm}}$
28. $\log_{(3(\lg 2 \lg 5 + \lg^2 2 + \lg 5))} (9+1)^{\log_{(10 \lg 10)} 9} = \underline{\hspace{2cm}}$
29. $\frac{\frac{1}{3} \lg (e^4)^3}{\frac{\lg 10}{5} \frac{\lg e^5}{\lg 3^{\log_3 10}}} = \underline{\hspace{2cm}}$
30. $5 \log_{(\frac{15}{4})} \left((12+13) \frac{1}{2} \right)^{\frac{1}{5}} - \log_5 (\frac{1}{2}) = \underline{\hspace{2cm}}$
31. $\frac{1}{\log_{(1+\frac{8}{3})} (5\frac{1}{3}) - \log_{(1+\frac{8}{3})} (\frac{1}{3})} = \underline{\hspace{2cm}}$
32. $\frac{\frac{\log_{(1+1)} 3^{\log_3 3}}{\log_{(1+1)} (1+1)}}{\log_{(1+1)} 3} = \underline{\hspace{2cm}}$
33. $\frac{\frac{\lg (\frac{64}{2}) + \lg 2}{\frac{1}{4} \lg 4^4}}{\log_{(2^{\log_2 10})}^{10}} = \underline{\hspace{2cm}}$
34. $\frac{1}{3} \log_{(\log_2 4)} (8 \times 2^1)^3 - \frac{1}{\log_{(2^1)} \log_2 4} = \underline{\hspace{2cm}}$
35. $\log_{(3^{\log_3 5})} (125(3+2)^1) - \log_{(2+3)} (3+2)^1 = \underline{\hspace{2cm}}$

36. $\frac{\lg\left(\frac{32 \times 2}{3 \times 3}\right) + \lg(3 \times 3)}{\frac{2 \log_2 4 \frac{1}{2}}{\log_2 10}} = \underline{\hspace{2cm}}$
37. $\log_{(e^{\ln 5})} \left(\frac{1}{5} \log_5 \left(\left(\frac{20}{2} \right)^{493+132} \right)^5 \right) = \underline{\hspace{2cm}}$
38. $\frac{\log_{(10^{\lg 5})} (3 \times 8) - \log_{(10^{\lg 5})} 8}{\frac{1}{4} \log_5 3^4} = \underline{\hspace{2cm}}$
39. $\frac{\log_7 \left(\frac{4}{\log_2 8} \right) + \log_7 \log_2 8}{\log_7 \left(\frac{4}{7^3} \right) + \log_7 7^3} = \underline{\hspace{2cm}}$
40. $\log_{\left(\frac{8}{2}+6\right)} \left(\frac{40000}{2} \frac{1}{4} \right) - \log_{\left(\frac{8}{2}+6\right)} \left(\frac{1}{4} \right) = \underline{\hspace{2cm}}$
41. $\frac{1}{3+2} 2 \log_{(9+e^{\ln 1})} \left((e^{\ln 1000})^5 \right)^{\frac{1}{2}} = \underline{\hspace{2cm}}$
42. $\frac{\log_2 (3(2+\log_2 4))}{\frac{\lg 3}{\lg 2}} - \log_{(2+1)} (2 + \log_2 4) = \underline{\hspace{2cm}}$
43. $2 \log_2 (2(1+1+3))^{\frac{1}{2}} - \log_2 \left(\frac{1+1+3}{2^3} \right) + \log_2 2^3 = \underline{\hspace{2cm}}$
44. $\frac{\frac{1}{\log_{10000} 2} \times 1^2}{\frac{\log_{(2^2)} 10}{\log_{(2^2)} 2} \times 1^2} = \underline{\hspace{2cm}}$
45. $\frac{\log_{(2 \times 2)} (3 \times 8) - \log_{(2 \times 2)} 8}{\log_{(2 \times 2)} (3 \times 8) - \log_{(2 \times 2)} 8} = \underline{\hspace{2cm}}$
46. $\frac{\log_{(2 \times 2)} (2 \times 6) - \log_{(2 \times 2)} 6}{\log_{(2 \times 2)} \log_3 9} = \underline{\hspace{2cm}}$
47. $\frac{\lg (10 \times 10^4) - \frac{1}{\log_{(10^4)} 10}}{\lg (10 \log_5 9) - \lg \log_5 9} = \underline{\hspace{2cm}}$
48. $\log_5 \left(\frac{5 \times 5}{\log_3 8} \right) + \log_5 \left(\frac{\log_3 8}{3 \times 2} \right) + \log_5 (3 \times 2) = \underline{\hspace{2cm}}$
49. $\frac{5 \log_5 \left(\frac{500}{3} \right)^{\frac{1}{5}}}{\frac{1}{\log \left(\frac{\log \left(5^{\log_5 5} \right)^5}{5} \right)^5}} = \underline{\hspace{2cm}}$
50. $\frac{\frac{1}{\log_{(e^4)} (2+3)} \log_2 2}{\log_{(3^{\log_3 5})} e \log_2 2} = \underline{\hspace{2cm}}$
51. $\frac{\log_3 (81(1+3+3-3))}{\log_3 (1+2+0 \times 2)} - \log_{(1+2)} (1+3) = \underline{\hspace{2cm}}$
52. $\frac{\frac{\ln (2 \times 2) - \ln 2}{\log_{(3^2)} (2 \log_2 2)}}{\frac{\log_{(3^2)} e}{\log_{(3^2)} e}} = \underline{\hspace{2cm}}$
53. $2 \frac{\log_{(2 \times 2)} (e^{\ln 3})^{\frac{1}{2}}}{\log_{(2 \times 2)} \left(\frac{12}{3} \right)} = \underline{\hspace{2cm}}$

$$54. \ln \left(\frac{e^{\frac{e^{\ln 2}}{2 \times 3}}}{e^1} \right) + \ln e^1 + \ln (2 \times 3) = \underline{\hspace{2cm}}$$

$$55. \frac{\log_{(1+1)} \left(\log_5 \left(\frac{5^{16}}{\log_2 8} \right) + \log_5 \log_2 8 \right)}{\log_{(1+1)} 4} = \underline{\hspace{2cm}}$$

$$56. \frac{\log_2 (10000 \times 2^1) - \log_2 2^1}{\log_2 (5^{\log_5 10} \log_3 8) - \log_2 \log_3 8} = \underline{\hspace{2cm}}$$

$$57. \frac{\log_3 \left(\frac{4}{\frac{9}{4} \times 2} \right)}{\log_3 \left(\frac{4}{4} \right) + \log_3 4} + \log_4 \left(\frac{9}{4} \times 2 \right) = \underline{\hspace{2cm}}$$

$$58. \frac{\frac{1}{\log(e^4) 10}}{\frac{\lg(2 \times 2)}{\log_2 e}} = \underline{\hspace{2cm}}$$

$$59. \frac{1}{\frac{\log_{(1+1)} e}{\log_{(1+1)} e^4 (\lg 2 \lg 2 + \lg 5 \lg 5 + 2 \lg 5 \lg 2)}} = \underline{\hspace{2cm}}$$

$$60. \log_5 (6255 (\lg 2 \lg 5 + \lg^2 5 + \lg 2)) - \log_5 \left(\frac{5}{2 \times 2} \right) + \log_5 (2 \times 2) = \underline{\hspace{2cm}}$$

$$61. \frac{\frac{\log_{(2 \times 2)} ((95 + 161) \times 5)}{\log_{(2 \times 2)} 4} \times 4 - \log_4 5 \times 4}{4} = \underline{\hspace{2cm}}$$

$$62. \log_4 \left(\frac{16}{\log_2 (8 \log_3 9) - \log_2 \log_3 9} \right) + \log_4 \log_{(\log_3 9)} 2^{\log_2 8} = \underline{\hspace{2cm}}$$

$$63. \frac{\frac{\log_2 e^{2 \log_2 2}}{\log_2 3}}{\frac{1}{\frac{\ln 5}{\log_5 \left(\frac{3}{\log_3 4} \right) + \log_5 \log_3 4}}} = \underline{\hspace{2cm}}$$

$$64. \frac{\frac{\ln \left(\frac{16}{4} \right)}{\log_{(2^2)} (1 + \log_2 5 + \log_5 2)}}{\log_{(2^2)} e} = \underline{\hspace{2cm}}$$

$$65. \frac{\log \left(3^{\log_3 5} \right)^4}{\log_5 \left(\frac{2(\lg 2 \lg 2 + \lg 5 \lg 5 + 2 \lg 5 \lg 2)}{5} \right) + \log_5 5} = \underline{\hspace{2cm}}$$

$$66. \log_3 \left(\frac{2^{\log_2 3} \frac{\log_7 16}{\log_7 2}}{3^1} \right) + \log_3 3^1 - \log_3 \left(\frac{\lg 16}{\lg 2} \right) = \underline{\hspace{2cm}}$$

$$67. \frac{\ln \left(5^{\log_5 1000} \log_2 4 \right) - \ln \log_2 4}{\ln \left(\frac{2 \times 15}{4} (3+2) \right) - \ln (3+2)} = \underline{\hspace{2cm}}$$

$$68. \log_{(5^{\log_5 4})} \left(\frac{64 \times 9}{\log_3 8} \right) + \log_{(5^{\log_5 4})} \log_3 8 - \frac{1}{\log_9 4} = \underline{\hspace{2cm}}$$

$$69. \log_5 \left(5^{\log_5 25} (e^{\ln 5})^3 \right) - \frac{1}{\log_{((e^{\ln 5})^3)} 5} = \underline{\hspace{2cm}}$$

$$70. \ln \left(\frac{e^4}{\frac{5(\lg 2 \lg 2 + \lg 5 \lg 5 + 2 \lg 5 \lg 2)}{2 \times 3}} \right) + \ln (2 \times 3) + \ln 5 = \underline{\hspace{2cm}}$$

$$71. \frac{\log_5 (e^4 \log_5 (2 \times 8))}{\log_5 e} - \ln \left(\frac{\lg (2 \times 8)}{\lg 5} \right) = \underline{\hspace{2cm}}$$

72. $\frac{\log\left(\frac{12}{2}\right)\left(\frac{64}{\log_3 8}\right) + \log\left(\frac{12}{2}\right)\log_3 8}{\log_3(2 + \log_3 9)} = \underline{\hspace{2cm}}$
73. $\log_3\left(\frac{3^{\frac{2\log_2 1}{3}}}{\log_2 4}\right) + \log_3 \log_2 4 - \log_3\left(\frac{2^{\log_2 1}}{3}\right) = \underline{\hspace{2cm}}$
74. $\log_{\left(\frac{8}{3}\right)}\left(\frac{4}{5}\right) + \log_{\left(\frac{8}{3}\right)}(5\log_5 9) - \log_{\left(\frac{8}{3}\right)}\log_5 9 = \underline{\hspace{2cm}}$
75. $\frac{\frac{\log_7 e^{\frac{12}{3}}}{\log_7 3}}{\frac{\log_3 3}{\log_{(3^2)} e}} = \underline{\hspace{2cm}}$
76. $\log_2(8 \times 5\log_2 9) - \log_2 \log_2 9 - \log_{(\log_2 4)}\left(\frac{5}{4}\right) + \log_{(\log_2 4)} 4 = \underline{\hspace{2cm}}$
77. $\frac{\lg\left(\frac{(1+1+2-2)^{\frac{1}{5}}}{3}\right)^5}{\frac{\log_{(3^2)} 3^{\log_3 2}}{\log_{(3^2)} 10}} = \underline{\hspace{2cm}}$
78. $\log_4\left(\frac{4}{2\log_2 2(2+1)}\right) + \frac{\lg(2\log_2 2(2+1))(2-1)}{\lg 4(2-1)} = \underline{\hspace{2cm}}$
79. $\frac{\frac{\ln 8}{\ln 3^{\log_3 10}}}{\frac{\log_{(3^2)} \log_3 \log_2 2^9}{\log_{(3^2)} e^{\ln 10}}} = \underline{\hspace{2cm}}$
80. $\log_2\left(\frac{\frac{8}{3}}{3(1+2)} \times 2^2\right) - \log_2 2^2 + \log_{\left(\frac{8}{2}\right)}(3(1+2)) = \underline{\hspace{2cm}}$
81. $\frac{\frac{\log_5(27(1+2)) - \log_5(1+2)}{\log_5\left(\frac{8}{2}\right)}}{\frac{1}{2^{\log_2 3}} \log_2 3^3} = \underline{\hspace{2cm}}$
82. $\frac{1}{5} \frac{\frac{1}{\log\left(\left(e^{3\log_3 3}\right)^5\right)^3}}{\log_3(e\log_3 8) - \log_3 \log_3 8} = \underline{\hspace{2cm}}$
83. $\frac{1}{\log_{\left(\frac{3}{5^{\log_5 6}}\right)}(3(\lg 2 \lg 2 + \lg 5 \lg 5 + 2 \lg 5 \lg 2))} + \log_{(10^{\lg 3})} 6 = \underline{\hspace{2cm}}$
84. $\ln\left(\frac{e^4(3+1)}{\log_3 4}\right) + \ln \log_3 4 - \frac{\log_7\left(\frac{3 \times 3 + 1 \times 3}{3}\right)}{\log_7 e} = \underline{\hspace{2cm}}$
85. $\frac{\log_2(\log_2 2 + \log_2 2)}{\frac{1}{\log_{\left(\frac{2}{3 \times 2}\right)}(1+1)} + \log_{(1+1)}(3 \times 2)} = \underline{\hspace{2cm}}$
86. $\frac{\log_3\left(\frac{3}{\left(\frac{12}{4}\right)^2}\right)}{\log_3\left(\frac{12}{4}\right)} + \log_{\left(\frac{12}{4}\right)}\left(\frac{12}{4}\right)^2 = \underline{\hspace{2cm}}$
87. $\frac{\log_{(2^2)}(93(\lg 2 \lg 5 + \lg^2 5 + \lg 2) \times 6) - \log_{(2^2)} 6}{\log_{(2^2)} 3} = \underline{\hspace{2cm}}$
88. $\frac{\frac{1}{5} \log_6 4^5}{\frac{1}{3} \log_6\left(\frac{\log_{(2^3)} 4^4}{(1+1)^{\log_{(2^3)} 2}}\right)^3} = \underline{\hspace{2cm}}$

$$89. \frac{\frac{\log(1+1)}{\log(1+1)^2} \cdot \frac{\log_3 e}{\log_3 2}}{\log_3 2} - \frac{\log_7 4}{\log_7 e} = \underline{\hspace{2cm}}$$

$$90. \frac{\frac{1}{4} \log_3 (e^2(2+3))^4}{\log_3 \left(\frac{e}{\log_2 9}\right) + \log_3 \log_2 9} - \ln(2+3) = \underline{\hspace{2cm}}$$

$$91. \log \left(\frac{\log_6 3}{10^{\log_6 5 \log_5 10}} \right) \left(\frac{3}{6} \right) + \log \left(\frac{\log_6 3}{10^{\log_6 5 \log_5 10}} \right) 6 = \underline{\hspace{2cm}}$$

$$92. 4 \log_{(10^{\lg 2})} \left(\frac{8}{2 \times 2} \right)^{\frac{1}{4}} + \frac{\frac{1}{\log(2 \times 2)^5}}{\frac{\log_3 10^{\lg 2}}{\log_3 5}} = \underline{\hspace{2cm}}$$

$$93. \log_3 \left(\frac{2+1}{23(\lg 2 \lg 2 + \lg 5 \lg 5 + 2 \lg 5 \lg 2)} \right) + \log_3 (23(\lg 2 \lg 2 + \lg 5 \lg 5 + 2 \lg 5 \lg 2)) = \underline{\hspace{2cm}}$$

$$94. \log_3 \left(\frac{10^{\log(2 \times 5) (9 \log_2 4) - \log(2 \times 5) \log_2 4}}{3 \times 3} \right) + \log_3 (3 \times 3) = \underline{\hspace{2cm}}$$

$$95. \frac{\frac{\log_2 125}{\log_5 5}}{5 \log_5 (5(\lg 2 \lg 2 + \lg 5 \lg 5 + 2 \lg 5 \lg 2)) \left(\frac{1}{4} \log_5 25^4 \right)^{\frac{1}{5}}} = \underline{\hspace{2cm}}$$

$$96. \frac{\log_2 \left(\frac{5 \times 25}{5^2 \log_2 2} \right)}{\log_2 (2+3)} + \log_5 \left(\frac{5^2 \log_2 2}{\log_2 4} \right) + \log_5 \log_2 4 = \underline{\hspace{2cm}}$$

$$97. \frac{\log_5 (25(2+3)) - \log_5 (2+3)}{\log_5 \left(\frac{5 \log_3 3}{5^3 \log_3 3} \right) + \frac{\log_5 5^3}{\log_5 5}} = \underline{\hspace{2cm}}$$

$$98. \frac{\log(2 \times 2 \times 1) 27}{\log(2 \times 2) \left(\frac{3(\lg 2 \lg 5 + \lg^2 2 + \lg 5)}{6} \right) + \log(2 \times 2) 6} = \underline{\hspace{2cm}}$$

$$99. \log_4 (256 \log_5 (2 \times 4)) - \frac{\frac{\log_2 (\log_5 (2 \times 4 \log_5 8) - \log_5 \log_5 8)}{\log_2 5}}{\log_5 4} = \underline{\hspace{2cm}}$$

$$100. \frac{\frac{\frac{\log_3 (11+16)}{\log_2 \left(\frac{10}{4} \right)}}{\log_2 3}}{\frac{\log_3 \log_3 3}{\frac{1}{3} \log(2^{\log_2 3}) 5^3}} = \underline{\hspace{2cm}} \quad \text{参考答案}$$

3; 2; 3; 1; 1; 4; 3; 2; 1; 2

1; 1; 1; 2; 3; 3; 3; 2; 2; 1

4; 2; 2; 1; 1; 3; 2; 2; 4; 2

1; 1; 3; 3; 3; 3; 4; 1; 1; 4

3; 1; 1; 4; 1; 1; 1; 2; 3; 4

4; 1; 1; 2; 2; 4; 1; 4; 4; 4

4; 2; 2; 2; 2; 1; 3; 3; 2; 4

4; 3; 1; 1; 4; 3; 1; 1; 3; 2

3; 3; 1; 4; 1; 1; 3; 1; 1; 2

1; 3; 1; 2; 3; 3; 2; 3; 4; 3